tests/fundamental_types.cpp
@@ -1,0 +1,42 @@
+// floating point
+float f;
+double d;
+long double ld;
+
+
+void dfun(float, double, long double)
+
+// integral
+char c;
+signed char sc;
+unsigned char uc;
+short s;
+signed short ss;
+unsigned short us;
+int i;
+signed int si;
+unsigned int ui;
+long l;
+signed long sl;
+unsigned long ul;
+long long ll;
+signed long long sll;
+unsigned long long ull;
+__int128_t i128;
+__uint128_t u128;
+
+void ifun(char,signed char, unsigned char, short, unsigned short, int, unsigned int, long, unsigned long, long long, unsigned long long, __int128_t, __uint128_t);
+
+// character
+wchar_t wc;
+#if 202002L <= __cplusplus
+char8_t c8;
+#endif
+#if 201102L <= __cplusplus
+char16_t c16;
+char32_t c32;
+#endif
+
+
+// boolean
+bool b;
